James C - memory is N -> Z again (broke StackToAssembly)

FlatStack/StackToAssembly.thy
@@ -79,11 +79,11 @@ primrec instruction_conv :: "flat_stack_instruction \<Rightarrow> b_assembly lis
 definition program_convert :: "flat_stack_program \<Rightarrow> b_assembly_program" where
   "program_convert \<Pi> = map_option (\<lambda>(\<pi>, s). (ABAssm 0 # concat (map instruction_conv \<pi>), s)) o \<Pi>"
 
-primrec stack_to_mem :: "int list \<Rightarrow> (int \<Rightarrow> int) \<Rightarrow> int \<Rightarrow> int" where
+primrec stack_to_mem :: "int list \<Rightarrow> (nat \<Rightarrow> int) \<Rightarrow> nat \<Rightarrow> int" where
   "stack_to_mem [] \<mu> k = (if k = 0 then 0 else \<mu> k)"
 | "stack_to_mem (i # is) \<mu> k = (
     if k = 0 then 1 + int (length is)
-    else if k = 1 + int (length is) then i
+    else if k = Suc (length is) then i
     else stack_to_mem is \<mu> k)"
 
 fun state_convert :: "flat_stack_state \<Rightarrow> b_assembly_state set" where
@@ -105,10 +105,10 @@ lemma [simp]: "stack_to_mem \<sigma> \<mu> 0 = int (length \<sigma>)"
 lemma [simp]: "k < 0 \<Longrightarrow> stack_to_mem \<sigma> \<mu> k = \<mu> k"
   by (induction \<sigma>) simp_all
 
-lemma stack_same: "k > 0 \<Longrightarrow> k \<le> int (length \<sigma>) \<Longrightarrow> stack_to_mem \<sigma> \<mu> k = stack_to_mem \<sigma> \<mu>' k"
+lemma stack_same: "k > 0 \<Longrightarrow> k \<le> length \<sigma> \<Longrightarrow> stack_to_mem \<sigma> \<mu> k = stack_to_mem \<sigma> \<mu>' k"
   by (induction \<sigma>) simp_all
 
-lemma [simp]: "k > int (length \<sigma>) \<Longrightarrow> stack_to_mem \<sigma> \<mu> k = \<mu> k"
+lemma [simp]: "k > length \<sigma> \<Longrightarrow> stack_to_mem \<sigma> \<mu> k = \<mu> k"
   by (induction \<sigma>) simp_all
 
 lemma [simp]: "(stack_to_mem (i1 # \<sigma>) \<mu>)(0 := int (length \<sigma>)) = 
@@ -121,21 +121,21 @@ lemma [simp]: "(stack_to_mem (i1 # \<sigma>) \<mu>)(0 := int (length \<sigma>)) 
       case True
         thus ?thesis by simp
       next case False
-        with stack_same show ?thesis by (cases "x > int (length \<sigma>)") simp_all
+        with stack_same show ?thesis by (cases "x > length \<sigma>") simp_all
       qed
   qed
 
-lemma [simp]: "(stack_to_mem (i2 # i3 # \<sigma>) \<mu>)(0 := 1 + int (length \<sigma>), 1 + int (length \<sigma>) := i1) =
+lemma [simp]: "(stack_to_mem (i2 # i3 # \<sigma>) \<mu>)(0 := 1 + int (length \<sigma>), Suc (length \<sigma>) := i1) =
     stack_to_mem (i1 # \<sigma>) (stack_to_mem (i2 # i3 # \<sigma>) \<mu>)"
   proof
     fix x
-    show "((stack_to_mem (i2 # i3 # \<sigma>) \<mu>)(0 := 1 + int (length \<sigma>), 1 + int (length \<sigma>) := i1)) x = 
+    show "((stack_to_mem (i2 # i3 # \<sigma>) \<mu>)(0 := 1 + int (length \<sigma>), Suc (length \<sigma>) := i1)) x = 
         stack_to_mem (i1 # \<sigma>) (stack_to_mem (i2 # i3 # \<sigma>) \<mu>) x" 
       proof (cases "x < 0")
       case True
         thus ?thesis by simp
       next case False
-        with stack_same show ?thesis by (cases "x > int (length \<sigma>)") simp_all
+        with stack_same show ?thesis by (cases "x > length \<sigma>") simp_all
       qed
   qed
 
@@ -165,15 +165,15 @@ lemma eval_stack_conv [simp]: "eval_flat_stack \<Pi> \<Sigma>\<^sub>S \<Sigma>\<
     let ?\<Sigma>\<^sub>A\<^sub>1 = "(?\<mu>, Some (?\<mu> 0), d, 
       [CBAssm {D} (Reg M), ABAssm 0, CBAssm {A, M} (Decr M), 
        CBAssm {M} DPlusM, ABAssm 0] @ ?\<pi>', s, \<omega>)"
-    let ?\<Sigma>\<^sub>A\<^sub>2 = "(?\<mu>, Some (?\<mu> 0), ?\<mu> (?\<mu> 0), 
+    let ?\<Sigma>\<^sub>A\<^sub>2 = "(?\<mu>, Some (?\<mu> 0), ?\<mu> (nat (?\<mu> 0)), 
       [ABAssm 0, CBAssm {A, M} (Decr M), CBAssm {M} DPlusM, ABAssm 0] @ ?\<pi>', s, \<omega>)"
-    let ?\<Sigma>\<^sub>A\<^sub>3 = "(?\<mu>, Some 0, ?\<mu> (?\<mu> 0), 
+    let ?\<Sigma>\<^sub>A\<^sub>3 = "(?\<mu>, Some 0, ?\<mu> (nat (?\<mu> 0)), 
       [CBAssm {A, M} (Decr M), CBAssm {M} DPlusM, ABAssm 0] @ ?\<pi>', s, \<omega>)"
-    let ?\<Sigma>\<^sub>A\<^sub>4 = "(?\<mu>(0 := ?\<mu> 0 - 1), Some (?\<mu> 0 - 1), ?\<mu> (?\<mu> 0), 
+    let ?\<Sigma>\<^sub>A\<^sub>4 = "(?\<mu>(0 := ?\<mu> 0 - 1), Some (?\<mu> 0 - 1), ?\<mu> (nat (?\<mu> 0)), 
       [CBAssm {M} DPlusM, ABAssm 0] @ ?\<pi>', s, \<omega>)"
-    let ?\<Sigma>\<^sub>A\<^sub>5 = "(stack_to_mem ((i1 + i2) # \<sigma>) ?\<mu>, Some (?\<mu> 0 - 1), ?\<mu> (?\<mu> 0), 
+    let ?\<Sigma>\<^sub>A\<^sub>5 = "(stack_to_mem ((i1 + i2) # \<sigma>) ?\<mu>, Some (?\<mu> 0 - 1), ?\<mu> (nat (?\<mu> 0)), 
       [ABAssm 0] @ ?\<pi>', s, \<omega>)"
-    let ?\<Sigma>\<^sub>A\<^sub>6 = "(stack_to_mem ((i1 + i2) # \<sigma>) ?\<mu>, Some 0, ?\<mu> (?\<mu> 0), ?\<pi>', s, \<omega>)"
+    let ?\<Sigma>\<^sub>A\<^sub>6 = "(stack_to_mem ((i1 + i2) # \<sigma>) ?\<mu>, Some 0, ?\<mu> (nat (?\<mu> 0)), ?\<pi>', s, \<omega>)"
     from M have step1: "eval_b_assembly (program_convert \<Pi>) \<Sigma>\<^sub>A = Some ?\<Sigma>\<^sub>A\<^sub>1" by simp
     have step2: "eval_b_assembly (program_convert \<Pi>) ?\<Sigma>\<^sub>A\<^sub>1 = Some ?\<Sigma>\<^sub>A\<^sub>2" by simp
     have step3: "eval_b_assembly (program_convert \<Pi>) ?\<Sigma>\<^sub>A\<^sub>2 = Some ?\<Sigma>\<^sub>A\<^sub>3" by simp
@@ -196,15 +196,15 @@ lemma eval_stack_conv [simp]: "eval_flat_stack \<Pi> \<Sigma>\<^sub>S \<Sigma>\<
     let ?\<Sigma>\<^sub>A\<^sub>1 = "(?\<mu>, Some (?\<mu> 0), d, 
       [CBAssm {D} (Reg M), ABAssm 0, 
        CBAssm {A, M} (Decr M), CBAssm {M} MMinusD, ABAssm 0] @ ?\<pi>', s, \<omega>)"
-    let ?\<Sigma>\<^sub>A\<^sub>2 = "(?\<mu>, Some (?\<mu> 0), ?\<mu> (?\<mu> 0), 
+    let ?\<Sigma>\<^sub>A\<^sub>2 = "(?\<mu>, Some (?\<mu> 0), ?\<mu> (nat (?\<mu> 0)), 
       [ABAssm 0, CBAssm {A, M} (Decr M), CBAssm {M} MMinusD, ABAssm 0] @ ?\<pi>', s, \<omega>)"
-    let ?\<Sigma>\<^sub>A\<^sub>3 = "(?\<mu>, Some 0, ?\<mu> (?\<mu> 0), 
+    let ?\<Sigma>\<^sub>A\<^sub>3 = "(?\<mu>, Some 0, ?\<mu> (nat (?\<mu> 0)), 
       [CBAssm {A, M} (Decr M), CBAssm {M} MMinusD, ABAssm 0] @ ?\<pi>', s, \<omega>)"
-    let ?\<Sigma>\<^sub>A\<^sub>4 = "(?\<mu>(0 := ?\<mu> 0 - 1), Some (?\<mu> 0 - 1), ?\<mu> (?\<mu> 0),
+    let ?\<Sigma>\<^sub>A\<^sub>4 = "(?\<mu>(0 := ?\<mu> 0 - 1), Some (?\<mu> 0 - 1), ?\<mu> (nat (?\<mu> 0)),
       [CBAssm {M} MMinusD, ABAssm 0] @ ?\<pi>', s, \<omega>)"
-    let ?\<Sigma>\<^sub>A\<^sub>5 = "(stack_to_mem ((i2 - i1) # \<sigma>) ?\<mu>, Some (?\<mu> 0 - 1), ?\<mu> (?\<mu> 0), 
+    let ?\<Sigma>\<^sub>A\<^sub>5 = "(stack_to_mem ((i2 - i1) # \<sigma>) ?\<mu>, Some (?\<mu> 0 - 1), ?\<mu> (nat (?\<mu> 0)), 
       [ABAssm 0] @ ?\<pi>', s, \<omega>)"
-    let ?\<Sigma>\<^sub>A\<^sub>6 = "(stack_to_mem ((i2 - i1) # \<sigma>) ?\<mu>, Some 0, ?\<mu> (?\<mu> 0), ?\<pi>', s, \<omega>)"
+    let ?\<Sigma>\<^sub>A\<^sub>6 = "(stack_to_mem ((i2 - i1) # \<sigma>) ?\<mu>, Some 0, ?\<mu> (nat (?\<mu> 0)), ?\<pi>', s, \<omega>)"
     from M have step1: "eval_b_assembly (program_convert \<Pi>) \<Sigma>\<^sub>A = Some ?\<Sigma>\<^sub>A\<^sub>1" by simp
     have step2: "eval_b_assembly (program_convert \<Pi>) ?\<Sigma>\<^sub>A\<^sub>1 = Some ?\<Sigma>\<^sub>A\<^sub>2" by simp
     have step3: "eval_b_assembly (program_convert \<Pi>) ?\<Sigma>\<^sub>A\<^sub>2 = Some ?\<Sigma>\<^sub>A\<^sub>3" by simp
@@ -224,14 +224,14 @@ lemma eval_stack_conv [simp]: "eval_flat_stack \<Pi> \<Sigma>\<^sub>S \<Sigma>\<
       [CBAssm {A} (Reg M), CBAssm {M} (NegR M), ABAssm 0] @ ?\<pi>', s, \<omega>)" by fastforce
     let ?\<mu> = "stack_to_mem (i1 # \<sigma>) \<mu>"
     let ?\<Sigma>\<^sub>A\<^sub>1 = "(?\<mu>, Some (?\<mu> 0), d, [CBAssm {M} (NegR M), ABAssm 0] @ ?\<pi>', s, \<omega>)"
-    let ?\<Sigma>\<^sub>A\<^sub>2 = "(?\<mu>(?\<mu> 0 := - ?\<mu> (?\<mu> 0)), Some (?\<mu> 0), d, [ABAssm 0] @ ?\<pi>', s, \<omega>)"
-    let ?\<Sigma>\<^sub>A\<^sub>3 = "(?\<mu>(?\<mu> 0 := - ?\<mu> (?\<mu> 0)), Some 0, d, ?\<pi>', s, \<omega>)"
+    let ?\<Sigma>\<^sub>A\<^sub>2 = "(?\<mu>(nat (?\<mu> 0) := - ?\<mu> (nat (?\<mu> 0))), Some (?\<mu> 0), d, [ABAssm 0] @ ?\<pi>', s, \<omega>)"
+    let ?\<Sigma>\<^sub>A\<^sub>3 = "(?\<mu>(nat (?\<mu> 0) := - ?\<mu> (nat (?\<mu> 0))), Some 0, d, ?\<pi>', s, \<omega>)"
     from M have step1: "eval_b_assembly (program_convert \<Pi>) \<Sigma>\<^sub>A = Some ?\<Sigma>\<^sub>A\<^sub>1" by simp
     have step2: "eval_b_assembly (program_convert \<Pi>) ?\<Sigma>\<^sub>A\<^sub>1 = Some ?\<Sigma>\<^sub>A\<^sub>2" by simp
     have "eval_b_assembly (program_convert \<Pi>) ?\<Sigma>\<^sub>A\<^sub>2 = Some ?\<Sigma>\<^sub>A\<^sub>3" by simp
     with iter_two iter_prestep step1 step2 have X:
       "iterate (eval_b_assembly (program_convert \<Pi>)) \<Sigma>\<^sub>A ?\<Sigma>\<^sub>A\<^sub>3" by fast
-    have "(stack_to_mem (i1 # \<sigma>) \<mu>)(1 + int (length \<sigma>) := - i1) = stack_to_mem (- i1 # \<sigma>) \<mu>" by auto
+    have "(stack_to_mem (i1 # \<sigma>) \<mu>)(1 + Suc (length \<sigma>) := - i1) = stack_to_mem (- i1 # \<sigma>) \<mu>" by auto
     hence "?\<Sigma>\<^sub>A\<^sub>3 \<in> state_convert ((-i1) # \<sigma>, \<pi>, s, \<omega>)" by auto
     with X show ?case by metis
   next case (evf_eq \<Pi> i1 i2 \<sigma> \<pi> s \<omega>)
@@ -247,56 +247,56 @@ lemma eval_stack_conv [simp]: "eval_flat_stack \<Pi> \<Sigma>\<^sub>S \<Sigma>\<
       [CBAssm {D} (Reg M), ABAssm 0, CBAssm {A, M} (Decr M), CBAssm {D} MMinusD, 
        IBAssm {EQ} [ABAssm 0, CBAssm {A} (Reg M), CBAssm {M} One] 
                    [ABAssm 0, CBAssm {A} (Reg M), CBAssm {M} Zero], ABAssm 0] @ ?\<pi>', s, \<omega>)"
-    let ?\<Sigma>\<^sub>A\<^sub>2 = "(?\<mu>, Some (?\<mu> 0), ?\<mu> (?\<mu> 0), 
+    let ?\<Sigma>\<^sub>A\<^sub>2 = "(?\<mu>, Some (?\<mu> 0), ?\<mu> (nat (?\<mu> 0)), 
       [ABAssm 0, CBAssm {A, M} (Decr M), CBAssm {D} MMinusD, 
        IBAssm {EQ} [ABAssm 0, CBAssm {A} (Reg M), CBAssm {M} One] 
                    [ABAssm 0, CBAssm {A} (Reg M), CBAssm {M} Zero], ABAssm 0] @ ?\<pi>', s, \<omega>)"
-    let ?\<Sigma>\<^sub>A\<^sub>3 = "(?\<mu>, Some 0, ?\<mu> (?\<mu> 0), 
+    let ?\<Sigma>\<^sub>A\<^sub>3 = "(?\<mu>, Some 0, ?\<mu> (nat (?\<mu> 0)), 
       [CBAssm {A, M} (Decr M), CBAssm {D} MMinusD, 
        IBAssm {EQ} [ABAssm 0, CBAssm {A} (Reg M), CBAssm {M} One] 
                    [ABAssm 0, CBAssm {A} (Reg M), CBAssm {M} Zero], ABAssm 0] @ ?\<pi>', s, \<omega>)"
-    let ?\<Sigma>\<^sub>A\<^sub>4 = "(?\<mu>(0 := ?\<mu> 0 - 1), Some (?\<mu> 0 - 1), ?\<mu> (?\<mu> 0), 
+    let ?\<Sigma>\<^sub>A\<^sub>4 = "(?\<mu>(0 := ?\<mu> 0 - 1), Some (?\<mu> 0 - 1), ?\<mu> (nat (?\<mu> 0)), 
       [CBAssm {D} MMinusD, IBAssm {EQ} [ABAssm 0, CBAssm {A} (Reg M), CBAssm {M} One] 
         [ABAssm 0, CBAssm {A} (Reg M), CBAssm {M} Zero], ABAssm 0] @ ?\<pi>', s, \<omega>)"
-    let ?\<Sigma>\<^sub>A\<^sub>5 = "(?\<mu>(0 := ?\<mu> 0 - 1), Some (?\<mu> 0 - 1), ?\<mu> (?\<mu> 0 - 1) - ?\<mu> (?\<mu> 0), 
+    let ?\<Sigma>\<^sub>A\<^sub>5 = "(?\<mu>(0 := ?\<mu> 0 - 1), Some (?\<mu> 0 - 1), ?\<mu> (nat (?\<mu> 0 - 1)) - ?\<mu> (nat (?\<mu> 0)), 
       [IBAssm {EQ} [ABAssm 0, CBAssm {A} (Reg M), CBAssm {M} One] 
                    [ABAssm 0, CBAssm {A} (Reg M), CBAssm {M} Zero], ABAssm 0] @ ?\<pi>', s, \<omega>)"
-    let ?\<Sigma>\<^sub>A\<^sub>6\<^sub>t = "(?\<mu>(0 := ?\<mu> 0 - 1), None, ?\<mu> (?\<mu> 0 - 1) - ?\<mu> (?\<mu> 0), 
+    let ?\<Sigma>\<^sub>A\<^sub>6\<^sub>t = "(?\<mu>(0 := ?\<mu> 0 - 1), None, ?\<mu> (nat (?\<mu> 0 - 1)) - ?\<mu> (nat (?\<mu> 0)), 
       [ABAssm 0, CBAssm {A} (Reg M), CBAssm {M} One, ABAssm 0] @ ?\<pi>', s, \<omega>)"
-    let ?\<Sigma>\<^sub>A\<^sub>7\<^sub>t = "(?\<mu>(0 := ?\<mu> 0 - 1), Some 0, ?\<mu> (?\<mu> 0 - 1) - ?\<mu> (?\<mu> 0), 
+    let ?\<Sigma>\<^sub>A\<^sub>7\<^sub>t = "(?\<mu>(0 := ?\<mu> 0 - 1), Some 0, ?\<mu> (nat (?\<mu> 0 - 1)) - ?\<mu> (nat (?\<mu> 0)), 
       [CBAssm {A} (Reg M), CBAssm {M} One, ABAssm 0] @ ?\<pi>', s, \<omega>)"
-    let ?\<Sigma>\<^sub>A\<^sub>8\<^sub>t = "(?\<mu>(0 := ?\<mu> 0 - 1), Some (?\<mu> 0 - 1), ?\<mu> (?\<mu> 0 - 1) - ?\<mu> (?\<mu> 0), 
+    let ?\<Sigma>\<^sub>A\<^sub>8\<^sub>t = "(?\<mu>(0 := ?\<mu> 0 - 1), Some (?\<mu> 0 - 1), ?\<mu> (nat (?\<mu> 0 - 1)) - ?\<mu> (nat (?\<mu> 0)), 
       [CBAssm {M} One, ABAssm 0] @ ?\<pi>', s, \<omega>)"
-    let ?\<Sigma>\<^sub>A\<^sub>6\<^sub>f = "(?\<mu>(0 := ?\<mu> 0 - 1), None, ?\<mu> (?\<mu> 0 - 1) - ?\<mu> (?\<mu> 0), 
+    let ?\<Sigma>\<^sub>A\<^sub>6\<^sub>f = "(?\<mu>(0 := ?\<mu> 0 - 1), None, ?\<mu> (nat (?\<mu> 0 - 1)) - ?\<mu> (nat (?\<mu> 0)), 
       [ABAssm 0, CBAssm {A} (Reg M), CBAssm {M} Zero, ABAssm 0] @ ?\<pi>', s, \<omega>)"
-    let ?\<Sigma>\<^sub>A\<^sub>7\<^sub>f = "(?\<mu>(0 := ?\<mu> 0 - 1), Some 0, ?\<mu> (?\<mu> 0 - 1) - ?\<mu> (?\<mu> 0), 
+    let ?\<Sigma>\<^sub>A\<^sub>7\<^sub>f = "(?\<mu>(0 := ?\<mu> 0 - 1), Some 0, ?\<mu> (nat (?\<mu> 0 - 1)) - ?\<mu> (nat (?\<mu> 0)), 
       [CBAssm {A} (Reg M), CBAssm {M} Zero, ABAssm 0] @ ?\<pi>', s, \<omega>)"
-    let ?\<Sigma>\<^sub>A\<^sub>8\<^sub>f = "(?\<mu>(0 := ?\<mu> 0 - 1), Some (?\<mu> 0 - 1), ?\<mu> (?\<mu> 0 - 1) - ?\<mu> (?\<mu> 0), 
+    let ?\<Sigma>\<^sub>A\<^sub>8\<^sub>f = "(?\<mu>(0 := ?\<mu> 0 - 1), Some (?\<mu> 0 - 1), ?\<mu> (nat (?\<mu> 0 - 1)) - ?\<mu> (nat (?\<mu> 0)), 
       [CBAssm {M} Zero, ABAssm 0] @ ?\<pi>', s, \<omega>)"
     let ?\<Sigma>\<^sub>A\<^sub>9 = "(stack_to_mem (unboolify (i2 = i1) # \<sigma>) ?\<mu>, Some (?\<mu> 0 - 1), 
-      ?\<mu> (?\<mu> 0 - 1) - ?\<mu> (?\<mu> 0), [ABAssm 0] @ ?\<pi>', s, \<omega>)"
+      ?\<mu> (nat (?\<mu> 0 - 1)) - ?\<mu> (nat (?\<mu> 0)), [ABAssm 0] @ ?\<pi>', s, \<omega>)"
     let ?\<Sigma>\<^sub>A\<^sub>1\<^sub>0 = "(stack_to_mem (unboolify (i2 = i1) # \<sigma>) ?\<mu>, Some 0, 
-      ?\<mu> (?\<mu> 0 - 1) - ?\<mu> (?\<mu> 0), ?\<pi>', s, \<omega>)"
+      ?\<mu> (nat (?\<mu> 0 - 1)) - ?\<mu> (nat (?\<mu> 0)), ?\<pi>', s, \<omega>)"
     from M have step1: "eval_b_assembly (program_convert \<Pi>) \<Sigma>\<^sub>A = Some ?\<Sigma>\<^sub>A\<^sub>1" by simp
     have step2: "eval_b_assembly (program_convert \<Pi>) ?\<Sigma>\<^sub>A\<^sub>1 = Some ?\<Sigma>\<^sub>A\<^sub>2" by simp
     have step3: "eval_b_assembly (program_convert \<Pi>) ?\<Sigma>\<^sub>A\<^sub>2 = Some ?\<Sigma>\<^sub>A\<^sub>3" by simp
     have step4: "eval_b_assembly (program_convert \<Pi>) ?\<Sigma>\<^sub>A\<^sub>3 = Some ?\<Sigma>\<^sub>A\<^sub>4" by (simp add: Let_def)
     have step5: "eval_b_assembly (program_convert \<Pi>) ?\<Sigma>\<^sub>A\<^sub>4 = Some ?\<Sigma>\<^sub>A\<^sub>5" by simp
-    have step6t: "?\<mu> (?\<mu> 0 - 1) = ?\<mu> (?\<mu> 0) \<Longrightarrow> 
+    have step6t: "?\<mu> (nat (?\<mu> 0 - 1)) = ?\<mu> (nat (?\<mu> 0)) \<Longrightarrow> 
       eval_b_assembly (program_convert \<Pi>) ?\<Sigma>\<^sub>A\<^sub>5 = Some ?\<Sigma>\<^sub>A\<^sub>6\<^sub>t" by simp
-    have step7t: "?\<mu> (?\<mu> 0 - 1) = ?\<mu> (?\<mu> 0) \<Longrightarrow> 
+    have step7t: "?\<mu> (nat (?\<mu> 0 - 1)) = ?\<mu> (nat (?\<mu> 0)) \<Longrightarrow> 
       eval_b_assembly (program_convert \<Pi>) ?\<Sigma>\<^sub>A\<^sub>6\<^sub>t = Some ?\<Sigma>\<^sub>A\<^sub>7\<^sub>t" by simp
-    have step8t: "?\<mu> (?\<mu> 0 - 1) = ?\<mu> (?\<mu> 0) \<Longrightarrow> 
+    have step8t: "?\<mu> (nat (?\<mu> 0 - 1)) = ?\<mu> (nat (?\<mu> 0)) \<Longrightarrow> 
       eval_b_assembly (program_convert \<Pi>) ?\<Sigma>\<^sub>A\<^sub>7\<^sub>t = Some ?\<Sigma>\<^sub>A\<^sub>8\<^sub>t" by simp
-    have step9t: "?\<mu> (?\<mu> 0 - 1) = ?\<mu> (?\<mu> 0) \<Longrightarrow> 
+    have step9t: "?\<mu> (nat (?\<mu> 0 - 1)) = ?\<mu> (nat (?\<mu> 0)) \<Longrightarrow> 
       eval_b_assembly (program_convert \<Pi>) ?\<Sigma>\<^sub>A\<^sub>8\<^sub>t = Some ?\<Sigma>\<^sub>A\<^sub>9" by simp
-    have step6f: "?\<mu> (?\<mu> 0 - 1) \<noteq> ?\<mu> (?\<mu> 0) \<Longrightarrow> 
+    have step6f: "?\<mu> (nat (?\<mu> 0 - 1)) \<noteq> ?\<mu> (nat (?\<mu> 0)) \<Longrightarrow> 
       eval_b_assembly (program_convert \<Pi>) ?\<Sigma>\<^sub>A\<^sub>5 = Some ?\<Sigma>\<^sub>A\<^sub>6\<^sub>f" by simp
-    have step7f: "?\<mu> (?\<mu> 0 - 1) \<noteq> ?\<mu> (?\<mu> 0) \<Longrightarrow> 
+    have step7f: "?\<mu> (nat (?\<mu> 0 - 1)) \<noteq> ?\<mu> (nat (?\<mu> 0)) \<Longrightarrow> 
       eval_b_assembly (program_convert \<Pi>) ?\<Sigma>\<^sub>A\<^sub>6\<^sub>f = Some ?\<Sigma>\<^sub>A\<^sub>7\<^sub>f" by simp
-    have step8f: "?\<mu> (?\<mu> 0 - 1) \<noteq> ?\<mu> (?\<mu> 0) \<Longrightarrow> 
+    have step8f: "?\<mu> (nat (?\<mu> 0 - 1)) \<noteq> ?\<mu> (nat (?\<mu> 0)) \<Longrightarrow> 
       eval_b_assembly (program_convert \<Pi>) ?\<Sigma>\<^sub>A\<^sub>7\<^sub>f = Some ?\<Sigma>\<^sub>A\<^sub>8\<^sub>f" by simp
-    have step9f: "?\<mu> (?\<mu> 0 - 1) \<noteq> ?\<mu> (?\<mu> 0) \<Longrightarrow> 
+    have step9f: "?\<mu> (nat (?\<mu> 0 - 1)) \<noteq> ?\<mu> (nat (?\<mu> 0)) \<Longrightarrow> 
       eval_b_assembly (program_convert \<Pi>) ?\<Sigma>\<^sub>A\<^sub>8\<^sub>f = Some ?\<Sigma>\<^sub>A\<^sub>9" by simp
     have step10: "eval_b_assembly (program_convert \<Pi>) ?\<Sigma>\<^sub>A\<^sub>9 = Some ?\<Sigma>\<^sub>A\<^sub>1\<^sub>0" by simp
     from iter_two iter_prestep step1 step2 step3 have 
@@ -304,7 +304,7 @@ lemma eval_stack_conv [simp]: "eval_flat_stack \<Pi> \<Sigma>\<^sub>S \<Sigma>\<
     with iter_two step4 step5 have Y: 
       "iterate (eval_b_assembly (program_convert \<Pi>)) \<Sigma>\<^sub>A ?\<Sigma>\<^sub>A\<^sub>5" by fast
     have "iterate (eval_b_assembly (program_convert \<Pi>)) ?\<Sigma>\<^sub>A\<^sub>5 ?\<Sigma>\<^sub>A\<^sub>1\<^sub>0"
-      proof (cases "?\<mu> (?\<mu> 0 - 1) = ?\<mu> (?\<mu> 0)")
+      proof (cases "?\<mu> (nat (?\<mu> 0 - 1)) = ?\<mu> (nat (?\<mu> 0))")
       case True
         with iter_two iter_prestep step6t step7t step8t have 
           "iterate (eval_b_assembly (program_convert \<Pi>)) ?\<Sigma>\<^sub>A\<^sub>5 ?\<Sigma>\<^sub>A\<^sub>8\<^sub>t" by fast
@@ -330,56 +330,56 @@ lemma eval_stack_conv [simp]: "eval_flat_stack \<Pi> \<Sigma>\<^sub>S \<Sigma>\<
       [CBAssm {D} (Reg M), ABAssm 0, CBAssm {A, M} (Decr M), CBAssm {D} MMinusD, 
        IBAssm {GT} [ABAssm 0, CBAssm {A} (Reg M), CBAssm {M} One] 
                    [ABAssm 0, CBAssm {A} (Reg M), CBAssm {M} Zero], ABAssm 0] @ ?\<pi>', s, \<omega>)"
-    let ?\<Sigma>\<^sub>A\<^sub>2 = "(?\<mu>, Some (?\<mu> 0), ?\<mu> (?\<mu> 0), 
+    let ?\<Sigma>\<^sub>A\<^sub>2 = "(?\<mu>, Some (?\<mu> 0), ?\<mu> (nat (?\<mu> 0)), 
       [ABAssm 0, CBAssm {A, M} (Decr M), CBAssm {D} MMinusD, 
        IBAssm {GT} [ABAssm 0, CBAssm {A} (Reg M), CBAssm {M} One] 
                    [ABAssm 0, CBAssm {A} (Reg M), CBAssm {M} Zero], ABAssm 0] @ ?\<pi>', s, \<omega>)"
-    let ?\<Sigma>\<^sub>A\<^sub>3 = "(?\<mu>, Some 0, ?\<mu> (?\<mu> 0), 
+    let ?\<Sigma>\<^sub>A\<^sub>3 = "(?\<mu>, Some 0, ?\<mu> (nat (?\<mu> 0)), 
       [CBAssm {A, M} (Decr M), CBAssm {D} MMinusD, 
        IBAssm {GT} [ABAssm 0, CBAssm {A} (Reg M), CBAssm {M} One] 
                    [ABAssm 0, CBAssm {A} (Reg M), CBAssm {M} Zero], ABAssm 0] @ ?\<pi>', s, \<omega>)"
-    let ?\<Sigma>\<^sub>A\<^sub>4 = "(?\<mu>(0 := ?\<mu> 0 - 1), Some (?\<mu> 0 - 1), ?\<mu> (?\<mu> 0), 
+    let ?\<Sigma>\<^sub>A\<^sub>4 = "(?\<mu>(0 := ?\<mu> 0 - 1), Some (?\<mu> 0 - 1), ?\<mu> (nat (?\<mu> 0)), 
       [CBAssm {D} MMinusD, IBAssm {GT} [ABAssm 0, CBAssm {A} (Reg M), CBAssm {M} One] 
         [ABAssm 0, CBAssm {A} (Reg M), CBAssm {M} Zero], ABAssm 0] @ ?\<pi>', s, \<omega>)"
-    let ?\<Sigma>\<^sub>A\<^sub>5 = "(?\<mu>(0 := ?\<mu> 0 - 1), Some (?\<mu> 0 - 1), ?\<mu> (?\<mu> 0 - 1) - ?\<mu> (?\<mu> 0), 
+    let ?\<Sigma>\<^sub>A\<^sub>5 = "(?\<mu>(0 := ?\<mu> 0 - 1), Some (?\<mu> 0 - 1), ?\<mu> (nat (?\<mu> 0 - 1)) - ?\<mu> (nat (?\<mu> 0)), 
       [IBAssm {GT} [ABAssm 0, CBAssm {A} (Reg M), CBAssm {M} One] 
                    [ABAssm 0, CBAssm {A} (Reg M), CBAssm {M} Zero], ABAssm 0] @ ?\<pi>', s, \<omega>)"
-    let ?\<Sigma>\<^sub>A\<^sub>6\<^sub>t = "(?\<mu>(0 := ?\<mu> 0 - 1), None, ?\<mu> (?\<mu> 0 - 1) - ?\<mu> (?\<mu> 0), 
+    let ?\<Sigma>\<^sub>A\<^sub>6\<^sub>t = "(?\<mu>(0 := ?\<mu> 0 - 1), None, ?\<mu> (nat (?\<mu> 0 - 1)) - ?\<mu> (nat (?\<mu> 0)), 
       [ABAssm 0, CBAssm {A} (Reg M), CBAssm {M} One, ABAssm 0] @ ?\<pi>', s, \<omega>)"
-    let ?\<Sigma>\<^sub>A\<^sub>7\<^sub>t = "(?\<mu>(0 := ?\<mu> 0 - 1), Some 0, ?\<mu> (?\<mu> 0 - 1) - ?\<mu> (?\<mu> 0), 
+    let ?\<Sigma>\<^sub>A\<^sub>7\<^sub>t = "(?\<mu>(0 := ?\<mu> 0 - 1), Some 0, ?\<mu> (nat (?\<mu> 0 - 1)) - ?\<mu> (nat (?\<mu> 0)), 
       [CBAssm {A} (Reg M), CBAssm {M} One, ABAssm 0] @ ?\<pi>', s, \<omega>)"
-    let ?\<Sigma>\<^sub>A\<^sub>8\<^sub>t = "(?\<mu>(0 := ?\<mu> 0 - 1), Some (?\<mu> 0 - 1), ?\<mu> (?\<mu> 0 - 1) - ?\<mu> (?\<mu> 0), 
+    let ?\<Sigma>\<^sub>A\<^sub>8\<^sub>t = "(?\<mu>(0 := ?\<mu> 0 - 1), Some (?\<mu> 0 - 1), ?\<mu> (nat (?\<mu> 0 - 1)) - ?\<mu> (nat (?\<mu> 0)), 
       [CBAssm {M} One, ABAssm 0] @ ?\<pi>', s, \<omega>)"
-    let ?\<Sigma>\<^sub>A\<^sub>6\<^sub>f = "(?\<mu>(0 := ?\<mu> 0 - 1), None, ?\<mu> (?\<mu> 0 - 1) - ?\<mu> (?\<mu> 0), 
+    let ?\<Sigma>\<^sub>A\<^sub>6\<^sub>f = "(?\<mu>(0 := ?\<mu> 0 - 1), None, ?\<mu> (nat (?\<mu> 0 - 1)) - ?\<mu> (nat (?\<mu> 0)), 
       [ABAssm 0, CBAssm {A} (Reg M), CBAssm {M} Zero, ABAssm 0] @ ?\<pi>', s, \<omega>)"
-    let ?\<Sigma>\<^sub>A\<^sub>7\<^sub>f = "(?\<mu>(0 := ?\<mu> 0 - 1), Some 0, ?\<mu> (?\<mu> 0 - 1) - ?\<mu> (?\<mu> 0), 
+    let ?\<Sigma>\<^sub>A\<^sub>7\<^sub>f = "(?\<mu>(0 := ?\<mu> 0 - 1), Some 0, ?\<mu> (nat (?\<mu> 0 - 1)) - ?\<mu> (nat (?\<mu> 0)), 
       [CBAssm {A} (Reg M), CBAssm {M} Zero, ABAssm 0] @ ?\<pi>', s, \<omega>)"
-    let ?\<Sigma>\<^sub>A\<^sub>8\<^sub>f = "(?\<mu>(0 := ?\<mu> 0 - 1), Some (?\<mu> 0 - 1), ?\<mu> (?\<mu> 0 - 1) - ?\<mu> (?\<mu> 0), 
+    let ?\<Sigma>\<^sub>A\<^sub>8\<^sub>f = "(?\<mu>(0 := ?\<mu> 0 - 1), Some (?\<mu> 0 - 1), ?\<mu> (nat (?\<mu> 0 - 1)) - ?\<mu> (nat (?\<mu> 0)), 
       [CBAssm {M} Zero, ABAssm 0] @ ?\<pi>', s, \<omega>)"
     let ?\<Sigma>\<^sub>A\<^sub>9 = "(stack_to_mem (unboolify (i2 > i1) # \<sigma>) ?\<mu>, Some (?\<mu> 0 - 1), 
-      ?\<mu> (?\<mu> 0 - 1) - ?\<mu> (?\<mu> 0), [ABAssm 0] @ ?\<pi>', s, \<omega>)"
+      ?\<mu> (nat (?\<mu> 0 - 1)) - ?\<mu> (nat (?\<mu> 0)), [ABAssm 0] @ ?\<pi>', s, \<omega>)"
     let ?\<Sigma>\<^sub>A\<^sub>1\<^sub>0 = "(stack_to_mem (unboolify (i2 > i1) # \<sigma>) ?\<mu>, Some 0, 
-      ?\<mu> (?\<mu> 0 - 1) - ?\<mu> (?\<mu> 0), ?\<pi>', s, \<omega>)"
+      ?\<mu> (nat (?\<mu> 0 - 1)) - ?\<mu> (nat (?\<mu> 0)), ?\<pi>', s, \<omega>)"
     from M have step1: "eval_b_assembly (program_convert \<Pi>) \<Sigma>\<^sub>A = Some ?\<Sigma>\<^sub>A\<^sub>1" by simp
     have step2: "eval_b_assembly (program_convert \<Pi>) ?\<Sigma>\<^sub>A\<^sub>1 = Some ?\<Sigma>\<^sub>A\<^sub>2" by simp
     have step3: "eval_b_assembly (program_convert \<Pi>) ?\<Sigma>\<^sub>A\<^sub>2 = Some ?\<Sigma>\<^sub>A\<^sub>3" by simp
     have step4: "eval_b_assembly (program_convert \<Pi>) ?\<Sigma>\<^sub>A\<^sub>3 = Some ?\<Sigma>\<^sub>A\<^sub>4" by (simp add: Let_def)
     have step5: "eval_b_assembly (program_convert \<Pi>) ?\<Sigma>\<^sub>A\<^sub>4 = Some ?\<Sigma>\<^sub>A\<^sub>5" by simp
-    have step6t: "?\<mu> (?\<mu> 0 - 1) > ?\<mu> (?\<mu> 0) \<Longrightarrow> 
+    have step6t: "?\<mu> (nat (?\<mu> 0 - 1)) > ?\<mu> (nat (?\<mu> 0)) \<Longrightarrow> 
       eval_b_assembly (program_convert \<Pi>) ?\<Sigma>\<^sub>A\<^sub>5 = Some ?\<Sigma>\<^sub>A\<^sub>6\<^sub>t" by simp
-    have step7t: "?\<mu> (?\<mu> 0 - 1) > ?\<mu> (?\<mu> 0) \<Longrightarrow> 
+    have step7t: "?\<mu> (nat (?\<mu> 0 - 1)) > ?\<mu> (nat (?\<mu> 0)) \<Longrightarrow> 
       eval_b_assembly (program_convert \<Pi>) ?\<Sigma>\<^sub>A\<^sub>6\<^sub>t = Some ?\<Sigma>\<^sub>A\<^sub>7\<^sub>t" by simp
-    have step8t: "?\<mu> (?\<mu> 0 - 1) > ?\<mu> (?\<mu> 0) \<Longrightarrow> 
+    have step8t: "?\<mu> (nat (?\<mu> 0 - 1)) > ?\<mu> (nat (?\<mu> 0)) \<Longrightarrow> 
       eval_b_assembly (program_convert \<Pi>) ?\<Sigma>\<^sub>A\<^sub>7\<^sub>t = Some ?\<Sigma>\<^sub>A\<^sub>8\<^sub>t" by simp
-    have step9t: "?\<mu> (?\<mu> 0 - 1) > ?\<mu> (?\<mu> 0) \<Longrightarrow> 
+    have step9t: "?\<mu> (nat (?\<mu> 0 - 1)) > ?\<mu> (nat (?\<mu> 0)) \<Longrightarrow> 
       eval_b_assembly (program_convert \<Pi>) ?\<Sigma>\<^sub>A\<^sub>8\<^sub>t = Some ?\<Sigma>\<^sub>A\<^sub>9" by simp
-    have step6f: "\<not> ?\<mu> (?\<mu> 0 - 1) > ?\<mu> (?\<mu> 0) \<Longrightarrow> 
+    have step6f: "\<not> ?\<mu> (nat (?\<mu> 0 - 1)) > ?\<mu> (nat (?\<mu> 0)) \<Longrightarrow> 
       eval_b_assembly (program_convert \<Pi>) ?\<Sigma>\<^sub>A\<^sub>5 = Some ?\<Sigma>\<^sub>A\<^sub>6\<^sub>f" by simp
-    have step7f: "\<not> ?\<mu> (?\<mu> 0 - 1) > ?\<mu> (?\<mu> 0) \<Longrightarrow> 
+    have step7f: "\<not> ?\<mu> (nat (?\<mu> 0 - 1)) > ?\<mu> (nat (?\<mu> 0)) \<Longrightarrow> 
       eval_b_assembly (program_convert \<Pi>) ?\<Sigma>\<^sub>A\<^sub>6\<^sub>f = Some ?\<Sigma>\<^sub>A\<^sub>7\<^sub>f" by simp
-    have step8f: "\<not> ?\<mu> (?\<mu> 0 - 1) > ?\<mu> (?\<mu> 0) \<Longrightarrow> 
+    have step8f: "\<not> ?\<mu> (nat (?\<mu> 0 - 1)) > ?\<mu> (nat (?\<mu> 0)) \<Longrightarrow> 
       eval_b_assembly (program_convert \<Pi>) ?\<Sigma>\<^sub>A\<^sub>7\<^sub>f = Some ?\<Sigma>\<^sub>A\<^sub>8\<^sub>f" by simp
-    have step9f: "\<not> ?\<mu> (?\<mu> 0 - 1) > ?\<mu> (?\<mu> 0) \<Longrightarrow> 
+    have step9f: "\<not> ?\<mu> (nat (?\<mu> 0 - 1)) > ?\<mu> (nat (?\<mu> 0)) \<Longrightarrow> 
       eval_b_assembly (program_convert \<Pi>) ?\<Sigma>\<^sub>A\<^sub>8\<^sub>f = Some ?\<Sigma>\<^sub>A\<^sub>9" by simp
     have step10: "eval_b_assembly (program_convert \<Pi>) ?\<Sigma>\<^sub>A\<^sub>9 = Some ?\<Sigma>\<^sub>A\<^sub>1\<^sub>0" by simp
     from iter_two iter_prestep step1 step2 step3 have 
@@ -387,7 +387,7 @@ lemma eval_stack_conv [simp]: "eval_flat_stack \<Pi> \<Sigma>\<^sub>S \<Sigma>\<
     with iter_two step4 step5 have Y: 
       "iterate (eval_b_assembly (program_convert \<Pi>)) \<Sigma>\<^sub>A ?\<Sigma>\<^sub>A\<^sub>5" by fast
     have "iterate (eval_b_assembly (program_convert \<Pi>)) ?\<Sigma>\<^sub>A\<^sub>5 ?\<Sigma>\<^sub>A\<^sub>1\<^sub>0"
-      proof (cases "?\<mu> (?\<mu> 0 - 1) > ?\<mu> (?\<mu> 0)")
+      proof (cases "?\<mu> (nat (?\<mu> 0 - 1)) > ?\<mu> (nat (?\<mu> 0))")
       case True
         with iter_two iter_prestep step6t step7t step8t have 
           "iterate (eval_b_assembly (program_convert \<Pi>)) ?\<Sigma>\<^sub>A\<^sub>5 ?\<Sigma>\<^sub>A\<^sub>8\<^sub>t" by fast
@@ -413,56 +413,56 @@ lemma eval_stack_conv [simp]: "eval_flat_stack \<Pi> \<Sigma>\<^sub>S \<Sigma>\<
       [CBAssm {D} (Reg M), ABAssm 0, CBAssm {A, M} (Decr M), CBAssm {D} MMinusD, 
        IBAssm {LT} [ABAssm 0, CBAssm {A} (Reg M), CBAssm {M} One] 
                    [ABAssm 0, CBAssm {A} (Reg M), CBAssm {M} Zero], ABAssm 0] @ ?\<pi>', s, \<omega>)"
-    let ?\<Sigma>\<^sub>A\<^sub>2 = "(?\<mu>, Some (?\<mu> 0), ?\<mu> (?\<mu> 0), 
+    let ?\<Sigma>\<^sub>A\<^sub>2 = "(?\<mu>, Some (?\<mu> 0), ?\<mu> (nat (?\<mu> 0)), 
       [ABAssm 0, CBAssm {A, M} (Decr M), CBAssm {D} MMinusD, 
        IBAssm {LT} [ABAssm 0, CBAssm {A} (Reg M), CBAssm {M} One] 
                    [ABAssm 0, CBAssm {A} (Reg M), CBAssm {M} Zero], ABAssm 0] @ ?\<pi>', s, \<omega>)"
-    let ?\<Sigma>\<^sub>A\<^sub>3 = "(?\<mu>, Some 0, ?\<mu> (?\<mu> 0), 
+    let ?\<Sigma>\<^sub>A\<^sub>3 = "(?\<mu>, Some 0, ?\<mu> (nat (?\<mu> 0)), 
       [CBAssm {A, M} (Decr M), CBAssm {D} MMinusD, 
        IBAssm {LT} [ABAssm 0, CBAssm {A} (Reg M), CBAssm {M} One] 
                    [ABAssm 0, CBAssm {A} (Reg M), CBAssm {M} Zero], ABAssm 0] @ ?\<pi>', s, \<omega>)"
-    let ?\<Sigma>\<^sub>A\<^sub>4 = "(?\<mu>(0 := ?\<mu> 0 - 1), Some (?\<mu> 0 - 1), ?\<mu> (?\<mu> 0), 
+    let ?\<Sigma>\<^sub>A\<^sub>4 = "(?\<mu>(0 := ?\<mu> 0 - 1), Some (?\<mu> 0 - 1), ?\<mu> (nat (?\<mu> 0)), 
       [CBAssm {D} MMinusD, IBAssm {LT} [ABAssm 0, CBAssm {A} (Reg M), CBAssm {M} One] 
         [ABAssm 0, CBAssm {A} (Reg M), CBAssm {M} Zero], ABAssm 0] @ ?\<pi>', s, \<omega>)"
-    let ?\<Sigma>\<^sub>A\<^sub>5 = "(?\<mu>(0 := ?\<mu> 0 - 1), Some (?\<mu> 0 - 1), ?\<mu> (?\<mu> 0 - 1) - ?\<mu> (?\<mu> 0), 
+    let ?\<Sigma>\<^sub>A\<^sub>5 = "(?\<mu>(0 := ?\<mu> 0 - 1), Some (?\<mu> 0 - 1), ?\<mu> (nat (?\<mu> 0 - 1)) - ?\<mu> (nat (?\<mu> 0)), 
       [IBAssm {LT} [ABAssm 0, CBAssm {A} (Reg M), CBAssm {M} One] 
                    [ABAssm 0, CBAssm {A} (Reg M), CBAssm {M} Zero], ABAssm 0] @ ?\<pi>', s, \<omega>)"
-    let ?\<Sigma>\<^sub>A\<^sub>6\<^sub>t = "(?\<mu>(0 := ?\<mu> 0 - 1), None, ?\<mu> (?\<mu> 0 - 1) - ?\<mu> (?\<mu> 0), 
+    let ?\<Sigma>\<^sub>A\<^sub>6\<^sub>t = "(?\<mu>(0 := ?\<mu> 0 - 1), None, ?\<mu> (nat (?\<mu> 0 - 1)) - ?\<mu> (nat (?\<mu> 0)), 
       [ABAssm 0, CBAssm {A} (Reg M), CBAssm {M} One, ABAssm 0] @ ?\<pi>', s, \<omega>)"
-    let ?\<Sigma>\<^sub>A\<^sub>7\<^sub>t = "(?\<mu>(0 := ?\<mu> 0 - 1), Some 0, ?\<mu> (?\<mu> 0 - 1) - ?\<mu> (?\<mu> 0), 
+    let ?\<Sigma>\<^sub>A\<^sub>7\<^sub>t = "(?\<mu>(0 := ?\<mu> 0 - 1), Some 0, ?\<mu> (nat (?\<mu> 0 - 1)) - ?\<mu> (nat (?\<mu> 0)), 
       [CBAssm {A} (Reg M), CBAssm {M} One, ABAssm 0] @ ?\<pi>', s, \<omega>)"
-    let ?\<Sigma>\<^sub>A\<^sub>8\<^sub>t = "(?\<mu>(0 := ?\<mu> 0 - 1), Some (?\<mu> 0 - 1), ?\<mu> (?\<mu> 0 - 1) - ?\<mu> (?\<mu> 0), 
+    let ?\<Sigma>\<^sub>A\<^sub>8\<^sub>t = "(?\<mu>(0 := ?\<mu> 0 - 1), Some (?\<mu> 0 - 1), ?\<mu> (nat (?\<mu> 0 - 1)) - ?\<mu> (nat (?\<mu> 0)), 
       [CBAssm {M} One, ABAssm 0] @ ?\<pi>', s, \<omega>)"
-    let ?\<Sigma>\<^sub>A\<^sub>6\<^sub>f = "(?\<mu>(0 := ?\<mu> 0 - 1), None, ?\<mu> (?\<mu> 0 - 1) - ?\<mu> (?\<mu> 0), 
+    let ?\<Sigma>\<^sub>A\<^sub>6\<^sub>f = "(?\<mu>(0 := ?\<mu> 0 - 1), None, ?\<mu> (nat (?\<mu> 0 - 1)) - ?\<mu> (nat (?\<mu> 0)), 
       [ABAssm 0, CBAssm {A} (Reg M), CBAssm {M} Zero, ABAssm 0] @ ?\<pi>', s, \<omega>)"
-    let ?\<Sigma>\<^sub>A\<^sub>7\<^sub>f = "(?\<mu>(0 := ?\<mu> 0 - 1), Some 0, ?\<mu> (?\<mu> 0 - 1) - ?\<mu> (?\<mu> 0), 
+    let ?\<Sigma>\<^sub>A\<^sub>7\<^sub>f = "(?\<mu>(0 := ?\<mu> 0 - 1), Some 0, ?\<mu> (nat (?\<mu> 0 - 1)) - ?\<mu> (nat (?\<mu> 0)), 
       [CBAssm {A} (Reg M), CBAssm {M} Zero, ABAssm 0] @ ?\<pi>', s, \<omega>)"
-    let ?\<Sigma>\<^sub>A\<^sub>8\<^sub>f = "(?\<mu>(0 := ?\<mu> 0 - 1), Some (?\<mu> 0 - 1), ?\<mu> (?\<mu> 0 - 1) - ?\<mu> (?\<mu> 0), 
+    let ?\<Sigma>\<^sub>A\<^sub>8\<^sub>f = "(?\<mu>(0 := ?\<mu> 0 - 1), Some (?\<mu> 0 - 1), ?\<mu> (nat (?\<mu> 0 - 1)) - ?\<mu> (nat (?\<mu> 0)), 
       [CBAssm {M} Zero, ABAssm 0] @ ?\<pi>', s, \<omega>)"
     let ?\<Sigma>\<^sub>A\<^sub>9 = "(stack_to_mem (unboolify (i2 < i1) # \<sigma>) ?\<mu>, Some (?\<mu> 0 - 1), 
-      ?\<mu> (?\<mu> 0 - 1) - ?\<mu> (?\<mu> 0), [ABAssm 0] @ ?\<pi>', s, \<omega>)"
+      ?\<mu> (nat (?\<mu> 0 - 1)) - ?\<mu> (nat (?\<mu> 0)), [ABAssm 0] @ ?\<pi>', s, \<omega>)"
     let ?\<Sigma>\<^sub>A\<^sub>1\<^sub>0 = "(stack_to_mem (unboolify (i2 < i1) # \<sigma>) ?\<mu>, Some 0, 
-      ?\<mu> (?\<mu> 0 - 1) - ?\<mu> (?\<mu> 0), ?\<pi>', s, \<omega>)"
+      ?\<mu> (nat (?\<mu> 0 - 1)) - ?\<mu> (nat (?\<mu> 0)), ?\<pi>', s, \<omega>)"
     from M have step1: "eval_b_assembly (program_convert \<Pi>) \<Sigma>\<^sub>A = Some ?\<Sigma>\<^sub>A\<^sub>1" by simp
     have step2: "eval_b_assembly (program_convert \<Pi>) ?\<Sigma>\<^sub>A\<^sub>1 = Some ?\<Sigma>\<^sub>A\<^sub>2" by simp
     have step3: "eval_b_assembly (program_convert \<Pi>) ?\<Sigma>\<^sub>A\<^sub>2 = Some ?\<Sigma>\<^sub>A\<^sub>3" by simp
     have step4: "eval_b_assembly (program_convert \<Pi>) ?\<Sigma>\<^sub>A\<^sub>3 = Some ?\<Sigma>\<^sub>A\<^sub>4" by (simp add: Let_def)
     have step5: "eval_b_assembly (program_convert \<Pi>) ?\<Sigma>\<^sub>A\<^sub>4 = Some ?\<Sigma>\<^sub>A\<^sub>5" by simp
-    have step6t: "?\<mu> (?\<mu> 0 - 1) < ?\<mu> (?\<mu> 0) \<Longrightarrow> 
+    have step6t: "?\<mu> (nat (?\<mu> 0 - 1)) < ?\<mu> (nat (?\<mu> 0)) \<Longrightarrow> 
       eval_b_assembly (program_convert \<Pi>) ?\<Sigma>\<^sub>A\<^sub>5 = Some ?\<Sigma>\<^sub>A\<^sub>6\<^sub>t" by simp
-    have step7t: "?\<mu> (?\<mu> 0 - 1) < ?\<mu> (?\<mu> 0) \<Longrightarrow> 
+    have step7t: "?\<mu> (nat (?\<mu> 0 - 1)) < ?\<mu> (nat (?\<mu> 0)) \<Longrightarrow> 
       eval_b_assembly (program_convert \<Pi>) ?\<Sigma>\<^sub>A\<^sub>6\<^sub>t = Some ?\<Sigma>\<^sub>A\<^sub>7\<^sub>t" by simp
-    have step8t: "?\<mu> (?\<mu> 0 - 1) < ?\<mu> (?\<mu> 0) \<Longrightarrow> 
+    have step8t: "?\<mu> (nat (?\<mu> 0 - 1)) < ?\<mu> (nat (?\<mu> 0)) \<Longrightarrow> 
       eval_b_assembly (program_convert \<Pi>) ?\<Sigma>\<^sub>A\<^sub>7\<^sub>t = Some ?\<Sigma>\<^sub>A\<^sub>8\<^sub>t" by simp
-    have step9t: "?\<mu> (?\<mu> 0 - 1) < ?\<mu> (?\<mu> 0) \<Longrightarrow> 
+    have step9t: "?\<mu> (nat (?\<mu> 0 - 1)) < ?\<mu> (nat (?\<mu> 0)) \<Longrightarrow> 
       eval_b_assembly (program_convert \<Pi>) ?\<Sigma>\<^sub>A\<^sub>8\<^sub>t = Some ?\<Sigma>\<^sub>A\<^sub>9" by simp
-    have step6f: "\<not> ?\<mu> (?\<mu> 0 - 1) < ?\<mu> (?\<mu> 0) \<Longrightarrow> 
+    have step6f: "\<not> ?\<mu> (nat (?\<mu> 0 - 1)) < ?\<mu> (nat (?\<mu> 0)) \<Longrightarrow> 
       eval_b_assembly (program_convert \<Pi>) ?\<Sigma>\<^sub>A\<^sub>5 = Some ?\<Sigma>\<^sub>A\<^sub>6\<^sub>f" by simp
-    have step7f: "\<not> ?\<mu> (?\<mu> 0 - 1) < ?\<mu> (?\<mu> 0) \<Longrightarrow> 
+    have step7f: "\<not> ?\<mu> (nat (?\<mu> 0 - 1)) < ?\<mu> (nat (?\<mu> 0)) \<Longrightarrow> 
       eval_b_assembly (program_convert \<Pi>) ?\<Sigma>\<^sub>A\<^sub>6\<^sub>f = Some ?\<Sigma>\<^sub>A\<^sub>7\<^sub>f" by simp
-    have step8f: "\<not> ?\<mu> (?\<mu> 0 - 1) < ?\<mu> (?\<mu> 0) \<Longrightarrow> 
+    have step8f: "\<not> ?\<mu> (nat (?\<mu> 0 - 1)) < ?\<mu> (nat (?\<mu> 0)) \<Longrightarrow> 
       eval_b_assembly (program_convert \<Pi>) ?\<Sigma>\<^sub>A\<^sub>7\<^sub>f = Some ?\<Sigma>\<^sub>A\<^sub>8\<^sub>f" by simp
-    have step9f: "\<not> ?\<mu> (?\<mu> 0 - 1) < ?\<mu> (?\<mu> 0) \<Longrightarrow> 
+    have step9f: "\<not> ?\<mu> (nat (?\<mu> 0 - 1)) < ?\<mu> (nat (?\<mu> 0)) \<Longrightarrow> 
       eval_b_assembly (program_convert \<Pi>) ?\<Sigma>\<^sub>A\<^sub>8\<^sub>f = Some ?\<Sigma>\<^sub>A\<^sub>9" by simp
     have step10: "eval_b_assembly (program_convert \<Pi>) ?\<Sigma>\<^sub>A\<^sub>9 = Some ?\<Sigma>\<^sub>A\<^sub>1\<^sub>0" by simp
     from iter_two iter_prestep step1 step2 step3 have 
@@ -470,7 +470,7 @@ lemma eval_stack_conv [simp]: "eval_flat_stack \<Pi> \<Sigma>\<^sub>S \<Sigma>\<
     with iter_two step4 step5 have Y: 
       "iterate (eval_b_assembly (program_convert \<Pi>)) \<Sigma>\<^sub>A ?\<Sigma>\<^sub>A\<^sub>5" by fast
     have "iterate (eval_b_assembly (program_convert \<Pi>)) ?\<Sigma>\<^sub>A\<^sub>5 ?\<Sigma>\<^sub>A\<^sub>1\<^sub>0"
-      proof (cases "?\<mu> (?\<mu> 0 - 1) < ?\<mu> (?\<mu> 0)")
+      proof (cases "?\<mu> (nat (?\<mu> 0 - 1)) < ?\<mu> (nat (?\<mu> 0))")
       case True
         with iter_two iter_prestep step6t step7t step8t have 
           "iterate (eval_b_assembly (program_convert \<Pi>)) ?\<Sigma>\<^sub>A\<^sub>5 ?\<Sigma>\<^sub>A\<^sub>8\<^sub>t" by fast
@@ -491,16 +491,16 @@ lemma eval_stack_conv [simp]: "eval_flat_stack \<Pi> \<Sigma>\<^sub>S \<Sigma>\<
     let ?\<mu> = "stack_to_mem (i1 # i2 # \<sigma>) \<mu>"
     let ?\<Sigma>\<^sub>A\<^sub>1 = "(?\<mu>, Some (?\<mu> 0), d, 
       [CBAssm {D} (Reg M), ABAssm 0, CBAssm {A, M} (Decr M), CBAssm {M} DAndM, ABAssm 0] @ ?\<pi>', s, \<omega>)"
-    let ?\<Sigma>\<^sub>A\<^sub>2 = "(?\<mu>, Some (?\<mu> 0), ?\<mu> (?\<mu> 0), 
+    let ?\<Sigma>\<^sub>A\<^sub>2 = "(?\<mu>, Some (?\<mu> 0), ?\<mu> (nat (?\<mu> 0)), 
       [ABAssm 0, CBAssm {A, M} (Decr M), CBAssm {M} DAndM, ABAssm 0] @ ?\<pi>', s, \<omega>)"
-    let ?\<Sigma>\<^sub>A\<^sub>3 = "(?\<mu>, Some 0, ?\<mu> (?\<mu> 0), 
+    let ?\<Sigma>\<^sub>A\<^sub>3 = "(?\<mu>, Some 0, ?\<mu> (nat (?\<mu> 0)), 
       [CBAssm {A, M} (Decr M), CBAssm {M} DAndM, ABAssm 0] @ ?\<pi>', s, \<omega>)"
-    let ?\<Sigma>\<^sub>A\<^sub>4 = "(?\<mu>(0 := ?\<mu> 0 - 1), Some (?\<mu> 0 - 1), ?\<mu> (?\<mu> 0), 
+    let ?\<Sigma>\<^sub>A\<^sub>4 = "(?\<mu>(0 := ?\<mu> 0 - 1), Some (?\<mu> 0 - 1), ?\<mu> (nat (?\<mu> 0)), 
       [CBAssm {M} DAndM, ABAssm 0] @ ?\<pi>', s, \<omega>)"
     let ?\<Sigma>\<^sub>A\<^sub>5 = "(stack_to_mem (unboolify (boolify i1 \<and> boolify i2) # \<sigma>) ?\<mu>, Some (?\<mu> 0 - 1), 
-      ?\<mu> (?\<mu> 0), [ABAssm 0] @ ?\<pi>', s, \<omega>)"
+      ?\<mu> (nat (?\<mu> 0)), [ABAssm 0] @ ?\<pi>', s, \<omega>)"
     let ?\<Sigma>\<^sub>A\<^sub>6 = "(stack_to_mem (unboolify (boolify i1 \<and> boolify i2) # \<sigma>) ?\<mu>, Some 0, 
-      ?\<mu> (?\<mu> 0), ?\<pi>', s, \<omega>)"
+      ?\<mu> (nat (?\<mu> 0)), ?\<pi>', s, \<omega>)"
     from M have step1: "eval_b_assembly (program_convert \<Pi>) \<Sigma>\<^sub>A = Some ?\<Sigma>\<^sub>A\<^sub>1" by simp
     have step2: "eval_b_assembly (program_convert \<Pi>) ?\<Sigma>\<^sub>A\<^sub>1 = Some ?\<Sigma>\<^sub>A\<^sub>2" by simp
     have step3: "eval_b_assembly (program_convert \<Pi>) ?\<Sigma>\<^sub>A\<^sub>2 = Some ?\<Sigma>\<^sub>A\<^sub>3" by simp
@@ -522,16 +522,16 @@ lemma eval_stack_conv [simp]: "eval_flat_stack \<Pi> \<Sigma>\<^sub>S \<Sigma>\<
     let ?\<mu> = "stack_to_mem (i1 # i2 # \<sigma>) \<mu>"
     let ?\<Sigma>\<^sub>A\<^sub>1 = "(?\<mu>, Some (?\<mu> 0), d, 
       [CBAssm {D} (Reg M), ABAssm 0, CBAssm {A, M} (Decr M), CBAssm {M} DOrM, ABAssm 0] @ ?\<pi>', s, \<omega>)"
-    let ?\<Sigma>\<^sub>A\<^sub>2 = "(?\<mu>, Some (?\<mu> 0), ?\<mu> (?\<mu> 0), 
+    let ?\<Sigma>\<^sub>A\<^sub>2 = "(?\<mu>, Some (?\<mu> 0), ?\<mu> (nat (?\<mu> 0)), 
       [ABAssm 0, CBAssm {A, M} (Decr M), CBAssm {M} DOrM, ABAssm 0] @ ?\<pi>', s, \<omega>)"
-    let ?\<Sigma>\<^sub>A\<^sub>3 = "(?\<mu>, Some 0, ?\<mu> (?\<mu> 0), 
+    let ?\<Sigma>\<^sub>A\<^sub>3 = "(?\<mu>, Some 0, ?\<mu> (nat (?\<mu> 0)), 
       [CBAssm {A, M} (Decr M), CBAssm {M} DOrM, ABAssm 0] @ ?\<pi>', s, \<omega>)"
-    let ?\<Sigma>\<^sub>A\<^sub>4 = "(?\<mu>(0 := ?\<mu> 0 - 1), Some (?\<mu> 0 - 1), ?\<mu> (?\<mu> 0), 
+    let ?\<Sigma>\<^sub>A\<^sub>4 = "(?\<mu>(0 := ?\<mu> 0 - 1), Some (?\<mu> 0 - 1), ?\<mu> (nat (?\<mu> 0)), 
       [CBAssm {M} DOrM, ABAssm 0] @ ?\<pi>', s, \<omega>)"
     let ?\<Sigma>\<^sub>A\<^sub>5 = "(stack_to_mem (unboolify (boolify i1 \<or> boolify i2) # \<sigma>) ?\<mu>, Some (?\<mu> 0 - 1), 
-      ?\<mu> (?\<mu> 0), [ABAssm 0] @ ?\<pi>', s, \<omega>)"
+      ?\<mu> (nat (?\<mu> 0)), [ABAssm 0] @ ?\<pi>', s, \<omega>)"
     let ?\<Sigma>\<^sub>A\<^sub>6 = "(stack_to_mem (unboolify (boolify i1 \<or> boolify i2) # \<sigma>) ?\<mu>, Some 0, 
-      ?\<mu> (?\<mu> 0), ?\<pi>', s, \<omega>)"
+      ?\<mu> (nat (?\<mu> 0)), ?\<pi>', s, \<omega>)"
     from M have step1: "eval_b_assembly (program_convert \<Pi>) \<Sigma>\<^sub>A = Some ?\<Sigma>\<^sub>A\<^sub>1" by simp
     have step2: "eval_b_assembly (program_convert \<Pi>) ?\<Sigma>\<^sub>A\<^sub>1 = Some ?\<Sigma>\<^sub>A\<^sub>2" by simp
     have step3: "eval_b_assembly (program_convert \<Pi>) ?\<Sigma>\<^sub>A\<^sub>2 = Some ?\<Sigma>\<^sub>A\<^sub>3" by simp
@@ -551,15 +551,15 @@ lemma eval_stack_conv [simp]: "eval_flat_stack \<Pi> \<Sigma>\<^sub>S \<Sigma>\<
       [CBAssm {A} (Reg M), CBAssm {M} (NotR M), ABAssm 0] @ ?\<pi>', s, \<omega>)" by fastforce
     let ?\<mu> = "stack_to_mem (i1 # \<sigma>) \<mu>"
     let ?\<Sigma>\<^sub>A\<^sub>1 = "(?\<mu>, Some (?\<mu> 0), d, [CBAssm {M} (NotR M), ABAssm 0] @ ?\<pi>', s, \<omega>)"
-    let ?\<Sigma>\<^sub>A\<^sub>2 = "(?\<mu>(?\<mu> 0 := unboolify (\<not> boolify (?\<mu> (?\<mu> 0)))), Some (?\<mu> 0), d, 
+    let ?\<Sigma>\<^sub>A\<^sub>2 = "(?\<mu>(nat (?\<mu> 0) := unboolify (\<not> boolify (?\<mu> (nat (?\<mu> 0))))), Some (?\<mu> 0), d, 
       [ABAssm 0] @ ?\<pi>', s, \<omega>)"
-    let ?\<Sigma>\<^sub>A\<^sub>3 = "(?\<mu>(?\<mu> 0 := unboolify (\<not> boolify (?\<mu> (?\<mu> 0)))), Some 0, d, ?\<pi>', s, \<omega>)"
+    let ?\<Sigma>\<^sub>A\<^sub>3 = "(?\<mu>(nat (?\<mu> 0) := unboolify (\<not> boolify (?\<mu> (nat (?\<mu> 0))))), Some 0, d, ?\<pi>', s, \<omega>)"
     from M have step1: "eval_b_assembly (program_convert \<Pi>) \<Sigma>\<^sub>A = Some ?\<Sigma>\<^sub>A\<^sub>1" by simp
     have step2: "eval_b_assembly (program_convert \<Pi>) ?\<Sigma>\<^sub>A\<^sub>1 = Some ?\<Sigma>\<^sub>A\<^sub>2" by simp
     have "eval_b_assembly (program_convert \<Pi>) ?\<Sigma>\<^sub>A\<^sub>2 = Some ?\<Sigma>\<^sub>A\<^sub>3" by simp
     with iter_two iter_prestep step1 step2 have X:
       "iterate (eval_b_assembly (program_convert \<Pi>)) \<Sigma>\<^sub>A ?\<Sigma>\<^sub>A\<^sub>3" by fast
-    have "(stack_to_mem (i1 # \<sigma>) \<mu>)(1 + int (length \<sigma>) := unboolify (\<not> boolify i1)) = 
+    have "(stack_to_mem (i1 # \<sigma>) \<mu>)(Suc (length \<sigma>) := unboolify (\<not> boolify i1)) = 
       stack_to_mem (unboolify (\<not> boolify i1) # \<sigma>) \<mu>" by auto
     hence "?\<Sigma>\<^sub>A\<^sub>3 \<in> state_convert (unboolify (\<not> boolify i1) # \<sigma>, \<pi>, s, \<omega>)" by auto
     with X show ?case by metis
@@ -571,11 +571,11 @@ lemma eval_stack_conv [simp]: "eval_flat_stack \<Pi> \<Sigma>\<^sub>S \<Sigma>\<
     let ?\<mu> = "stack_to_mem (i1 # \<sigma>) \<mu>"
     let ?\<Sigma>\<^sub>A\<^sub>1 = "(?\<mu>, Some (?\<mu> 0), d, 
       [CBAssm {D} (Reg M), PBAssm, ABAssm 0, CBAssm {M} (Decr M)] @ ?\<pi>', s, \<omega>)"
-    let ?\<Sigma>\<^sub>A\<^sub>2 = "(?\<mu>, Some (?\<mu> 0), ?\<mu> (?\<mu> 0), [PBAssm, ABAssm 0, CBAssm {M} (Decr M)] @ ?\<pi>', s, \<omega>)"
-    let ?\<Sigma>\<^sub>A\<^sub>3 = "(?\<mu>, Some (?\<mu> 0), ?\<mu> (?\<mu> 0), 
-      [ABAssm 0, CBAssm {M} (Decr M)] @ ?\<pi>', s, ?\<mu> (?\<mu> 0) # \<omega>)"
-    let ?\<Sigma>\<^sub>A\<^sub>4 = "(?\<mu>, Some 0, ?\<mu> (?\<mu> 0), [CBAssm {M} (Decr M)] @ ?\<pi>', s, ?\<mu> (?\<mu> 0) # \<omega>)"
-    let ?\<Sigma>\<^sub>A\<^sub>5 = "(?\<mu>(0 := ?\<mu> 0 - 1), Some 0, ?\<mu> (?\<mu> 0), ?\<pi>', s, ?\<mu> (?\<mu> 0) # \<omega>)"
+    let ?\<Sigma>\<^sub>A\<^sub>2 = "(?\<mu>, Some (?\<mu> 0), ?\<mu> (nat (?\<mu> 0)), [PBAssm, ABAssm 0, CBAssm {M} (Decr M)] @ ?\<pi>', s, \<omega>)"
+    let ?\<Sigma>\<^sub>A\<^sub>3 = "(?\<mu>, Some (?\<mu> 0), ?\<mu> (nat (?\<mu> 0)), 
+      [ABAssm 0, CBAssm {M} (Decr M)] @ ?\<pi>', s, ?\<mu> (nat (?\<mu> 0)) # \<omega>)"
+    let ?\<Sigma>\<^sub>A\<^sub>4 = "(?\<mu>, Some 0, ?\<mu> (nat (?\<mu> 0)), [CBAssm {M} (Decr M)] @ ?\<pi>', s, ?\<mu> (nat (?\<mu> 0)) # \<omega>)"
+    let ?\<Sigma>\<^sub>A\<^sub>5 = "(?\<mu>(0 := ?\<mu> 0 - 1), Some 0, ?\<mu> (nat (?\<mu> 0)), ?\<pi>', s, ?\<mu> (nat (?\<mu> 0)) # \<omega>)"
     from M have step1: "eval_b_assembly (program_convert \<Pi>) \<Sigma>\<^sub>A = Some ?\<Sigma>\<^sub>A\<^sub>1" by simp
     have step2: "eval_b_assembly (program_convert \<Pi>) ?\<Sigma>\<^sub>A\<^sub>1 = Some ?\<Sigma>\<^sub>A\<^sub>2" by simp
     have step3: "eval_b_assembly (program_convert \<Pi>) ?\<Sigma>\<^sub>A\<^sub>2 = Some ?\<Sigma>\<^sub>A\<^sub>3" by simp
